before finite addon

src/computational_monads/simulation_semantics/constructions/logging/caching_oracle2.lean
@@ -21,7 +21,7 @@ This is used by being composed with other oracles, such as in `random_oracle`.
 
 open oracle_comp oracle_spec query_cache
 open prod (fst) (snd)
-open_locale ennreal
+open_locale ennreal big_operators
 
 variables {α β γ δ : Type} {spec spec' : oracle_spec}
 
@@ -70,93 +70,441 @@ begin
   pairwise_dist_equiv,
 end
 
-lemma fork_thing (oa : oracle_comp spec α)
-  (i : spec.ι) (f : α × query_cache spec → query_cache spec)
-  (x : α) (cache : query_cache spec) :
-  ⁅= (x, x) | simulate' cachingₛₒ oa cache ×ₘ simulate' cachingₛₒ oa cache⁆ ≤
-    ⁅= (x, x) | do {z ← simulate cachingₛₒ oa cache,
-      z' ← simulate' cachingₛₒ oa (f z), return (z.1, z')}⁆ :=
+lemma shorter (oa : oracle_comp spec α) --(s : query_cache spec)
+  (f : α × query_cache spec → query_cache spec)
+  (hf : ∀ z, ∅ ≤ f z ∧ f z ≤ z.2)
+  (z : α × query_cache spec)
+  (hz : z ∈ (simulate cachingₛₒ oa ∅).support) :
+  ⁅= z | simulate cachingₛₒ oa ∅⁆ ≤
+    ⁅= z | simulate cachingₛₒ oa (f z)⁆ :=
 begin
+  induction oa using oracle_comp.induction_on
+    with α a α β oa ob hoa hob i' t' generalizing f,
+  {
+    rw [mem_support_simulate_return_iff] at hz,
+    have : f z = ∅ := le_antisymm (hz.2 ▸ (hf z).2) (hf z).1,
+    exact le_of_eq (this ▸ rfl)
+  },
+  {
+    simp only [] at hoa hob,
+    simp [prob_output_simulate'_bind_eq_tsum_tsum],
+
+    refine ennreal.tsum_le_tsum (λ x, ennreal.tsum_le_tsum (λ s', _)),
+    specialize hoa (x, s'),
+    sorry,
+  },
+  {
+    sorry,
+  }
+end
+
+-- #check antitone
+
+
+def substitute_cache (cache : query_cache spec) :
+  Π {α : Type}, oracle_comp spec α → oracle_comp spec α
+| _ (pure' α a) := return a
+| _ (bind' α β oa ob) := (substitute_cache oa) >>= (λ x, substitute_cache (ob x))
+| _ (query i t) := if cache.is_cached i t then
+  return ((cache.lookup i t).get_or_else default) else query i t
+
+/-- Extra choices to be made while running a computation to get from an
+initial cache of `s` to a cache of `cache` (assuming it's possible to do so)-/
+noncomputable def extra_choices (s cache : query_cache spec) :
+  Π {α : Type}, oracle_comp spec α → finset (Σ (i : spec.ι), spec.domain i)
+| _ (pure' α a) := ∅
+| _ (bind' α β oa ob) := (extra_choices oa) ∪ ((substitute_cache s oa).fin_support.bUnion (λ x, extra_choices (ob x)))
+| _ (query i t) := if s.is_fresh i t then {⟨i, t⟩} else ∅
+
+lemma extra_choices_return (s cache : query_cache spec) (x : α) :
+  extra_choices s cache (return x) = ∅ := rfl
+
+lemma extra_choices_bind (s cache : query_cache spec) (oa : oracle_comp spec α)
+  (ob : α → oracle_comp spec β) : extra_choices s cache (oa >>= ob) = (extra_choices s cache oa) ∪
+    ((substitute_cache s oa).fin_support.bUnion (λ x, extra_choices s cache (ob x))):=
+begin
+  rw [← bind'_eq_bind, extra_choices],
+end
+
+lemma extra_choices_query (s cache : query_cache spec) (i : spec.ι) (t : spec.domain i) :
+  extra_choices s cache (query i t) =
+    if s.is_fresh i t then {⟨i, t⟩} else ∅ := rfl
+
+theorem hope (oa : oracle_comp spec α) (s cache : query_cache spec) (hs : s ≤ cache)
+  (x : α) (hx : (x, cache) ∈ (simulate cachingₛₒ oa s).support) :
+  ⁅= (x, cache) | simulate cachingₛₒ oa s⁆ =
+    (extra_choices s cache oa).prod (λ i, (fintype.card $ spec.range i.1)⁻¹) :=
+begin
+  induction oa using oracle_comp.induction_on
+    with α a α β oa ob hoa hob i t generalizing s cache,
+  {
+    rw [extra_choices_return, finset.prod_empty, simulate_return,
+      prob_output_return_eq_one_iff],
+    rwa [simulate_return, mem_support_return_iff] at hx,
+  },
+  {
+    rw [extra_choices_bind, finset.prod_union sorry],
+    rw [prob_output_simulate_bind_eq_tsum_tsum],
+  },
+  {
+    rw [extra_choices_query],
+    split_ifs with h,
+    {
+      rw [finset.prod_singleton, simulate_query, apply_eq],
+      rw [simulate_query, apply_eq] at hx,
+      simp [h] at hx ⊢,
+      rw [← hx],
+      refine trans (prob_output_bind_return_eq_single' _ _ _ x rfl _) _,
+      refine λ _ _ h', (prod.eq_iff_fst_eq_snd_eq.1 h').1,
+      rw [prob_output_query_eq_inv],
+    },
+    {
+      rw [finset.prod_empty],
+      rw [not_is_fresh_iff_is_cached] at h,
+      simp [h, simulate_query, apply_eq] at ⊢ hx,
+      intros x' s' hx' hs',
+      refine ⟨hx'.trans hx.1.symm, hs'.trans hx.2.symm⟩,
+    }
+  }
+end
+
+-- theorem testing (s cache : query_cache spec) ()
+
+-- lemma exists_list (oa : oracle_comp spec α) (s cache : query_cache spec)
+--   (z : α) :
+--   ∃ (qs : list spec.ι), ⁅= (z, cache) | simulate cachingₛₒ oa s⁆ =
+--     (qs.map (λ i, )) :=
+-- begin
+
+-- end
+
+lemma output_eq_of_state_eq (oa : oracle_comp spec α)
+  (s s' : query_cache spec) (hs : s ≤ s')
+  (x x' : α) (cache : query_cache spec)
+  (h : (x, cache) ∈ (simulate cachingₛₒ oa s).support)
+  (h' : (x', cache) ∈ (simulate cachingₛₒ oa s).support) :
+  x = x' :=
+begin
+  induction oa using oracle_comp.induction_on
+    with α a α β oa ob hoa hob i t generalizing s cache,
+  {
+    simp at h h',
+    simp [h.1, h'.1]
+  },
+  {
+    rw [mem_support_simulate_bind_iff] at h h',
+    obtain ⟨a, s, hs, hxa⟩ := h,
+    obtain ⟨a', s', hs', hxa'⟩ := h',
+    specialize hoa a a',
+    specialize hob a x x',
+  }
+end
+
+-- lemma prob_output_mono_bot (oa : oracle_comp spec α) (s : query_cache spec)
+--   (z : α × query_cache spec) (hz : s ≤ z.2) :
+--   ⁅= z | simulate cachingₛₒ oa ∅⁆ ≤ ⁅= z | simulate cachingₛₒ oa s⁆ :=
+-- begin
+--   induction oa using oracle_comp.induction_on
+--     with α a α β oa ob hoa hob i t generalizing s hz,
+
+--   {
+--     sorry,
+--   },
+--   {
+--     -- simp only [] at hoa hob,
+--     simp only [simulate_bind],
+--     simp only [prob_output_bind_eq_tsum, ennreal.tsum_prod'],
+--     refine ennreal.tsum_le_tsum (λ x, _),
+
+
+--   }
+-- end
+
+lemma maybe (oa : oracle_comp spec α) (ob : α → oracle_comp spec β)
+  (s : query_cache spec) (z : β) (cache : query_cache spec)
+  (hz : (z, cache) ∈ (simulate cachingₛₒ (oa >>= ob) s).support) :
+  ∃! (y : α × query_cache spec), y ∈ (simulate cachingₛₒ oa s).support ∧
+    (z, cache) ∈ (simulate cachingₛₒ (ob y.1) y.2).support :=
+begin
+  rw [mem_support_simulate_bind_iff] at hz,
+  obtain ⟨x, s', hx, hs'⟩ := hz,
+  refine ⟨(x, s'), ⟨hx, hs'⟩, _⟩,
+  rintro ⟨x', s''⟩ ⟨hx', hx''⟩,
   sorry,
 end
 
+
+lemma support_antitone (oa : oracle_comp spec α) (s s' : query_cache spec)
+  (hs : s ≤ s') : (simulate' cachingₛₒ oa s').support ⊆ (simulate' cachingₛₒ oa s).support :=
+begin
+  induction oa using oracle_comp.induction_on
+    with α a α β oa ob hoa hob i t generalizing s s',
+  {
+    -- rw [simulate_return, simulate_return],
+    simp,
+  },
+  sorry,
+  sorry,
+end
+
+lemma prob_output_mono (oa : oracle_comp spec α) (s s' : query_cache spec)
+  (hs : s ≤ s') (z : α × query_cache spec) (hz : s' ≤ z.2) :
+  ⁅= z | simulate cachingₛₒ oa s⁆ ≤ ⁅= z | simulate cachingₛₒ oa s'⁆ :=
+begin
+  by_cases h : z ∈ (simulate cachingₛₒ oa s').support,
+  {
+    have h' : z ∈ (simulate cachingₛₒ oa s).support := sorry,
+  }
+
+
+  -- induction oa using oracle_comp.induction_on
+  --   with α a α β oa ob hoa hob i t generalizing s s',
+  -- {
+  --   rw [simulate_return, simulate_return],
+  --   by_cases h : z = (a, s'),
+  --   {
+  --     simp [h],
+  --   },
+  --   {
+  --     have : z ≠ (a, s) := sorry,
+  --     rw [(prob_output_return_eq_zero_iff _ _ _).2 h,
+  --       (prob_output_return_eq_zero_iff _ _ _).2 this],
+  --     refine le_rfl,
+  --   }
+  -- },
+  -- {
+  --   simp only [simulate_bind],
+  --   simp only [prob_output_bind_eq_tsum],
+  --   simp only [ennreal.tsum_prod'],
+  --   -- simp_rw [@ennreal.tsum_comm α],
+  --   refine ennreal.tsum_le_tsum (λ x, _),
+
+
+  --   sorry,
+
+
+
+  -- },
+  -- {
+  --   simp only [simulate_query, apply_eq],
+  --   by_cases ht : s.is_fresh i t,
+  --   {
+  --     by_cases ht' : s'.is_fresh i t,
+  --     {
+  --       simp [ht, ht'],
+  --     }
+  --   }
+  -- }
+end
+
+
+
+-- lemma fork_thing_harder (oa : oracle_comp spec α)  (s : query_cache spec)
+--   (f : α × query_cache spec → query_cache spec)
+--   (hf : ∀ z, s ≤ f z ∧ f z ≤ z.2) (z : α × query_cache spec) :
+--   ⁅= (z, z) | do {z1 ← simulate cachingₛₒ oa s,
+--       z2 ← simulate cachingₛₒ oa s, return (z1, z2)}⁆ ≤
+--     ⁅= (z, z) | do {z1 ← simulate cachingₛₒ oa s,
+--       z2 ← simulate cachingₛₒ oa (f z1), return (z1, z2)}⁆ :=
+-- begin
+--   induction oa using oracle_comp.induction_on
+--     with α a α β oa ob hoa hob i t generalizing s f,
+--   {
+--     have : f (a, s) = s := sorry,
+--     simp [simulate_return, this],
+--   },
+--   {
+--     calc ⁅= (z, z) | do {z1 ← simulate cachingₛₒ (oa >>= ob) s,
+--         z2 ← simulate cachingₛₒ (oa >>= ob) s, return (z1, z2)}⁆ =
+--       ⁅= (z, z) | do {x1 ← simulate cachingₛₒ oa s,
+--         z1 ← simulate cachingₛₒ (ob x1.1) x1.2,
+--         x2 ← simulate cachingₛₒ oa s,
+--         z2 ← simulate cachingₛₒ (ob x2.1) x2.2,
+--         return (z1, z2)}⁆ : sorry
+
+--       ... ≤ ⁅= (z, z) | do {x1 ← simulate cachingₛₒ oa s,
+--         z1 ← simulate cachingₛₒ (ob x1.1) x1.2,
+--         x2 ← simulate cachingₛₒ oa (f z1),
+--         z2 ← simulate cachingₛₒ (ob x2.1) x2.2,
+--         return (z1, z2)}⁆ : sorry
+--       ... = ⁅= (z, z) | do {z1 ← simulate cachingₛₒ (oa >>= ob) s,
+--         z2 ← simulate cachingₛₒ (oa >>= ob) (f z1), return (z1, z2)}⁆ : sorry
+
+--   },
+--   sorry,
+-- end
+
+-- lemma fork_thing (oa : oracle_comp spec α)  (s : query_cache spec)
+--   (f : α × query_cache spec → query_cache spec)
+--   (hf : ∀ z, s ≤ f z ∧ f z ≤ z.2) (x : α) :
+--   ⁅= (x, x) | do {simulate' cachingₛₒ oa s ×ₘ simulate' cachingₛₒ oa s}⁆ ≤
+--     ⁅= (x, x) | do {z ← simulate cachingₛₒ oa s,
+--       z' ← simulate' cachingₛₒ oa (f z), return (z.1, z')}⁆ :=
+-- begin
+--   rw [product.def],
+--   -- refine le_trans (le_of_eq $ prob_output_product _ _ (x, x)) _,
+--   induction oa using oracle_comp.induction_on
+--     with α a α β oa ob hoa hob i t generalizing s f,
+--   {
+--     refine le_of_eq (dist_equiv.prob_output_eq (symm (trans
+--       (simulate_bind_dist_equiv_simulate'_bind _ _ _ s s (λ _ _, _)) _)) _); pairwise_dist_equiv },
+--   {
+--     simp only [] at hoa hob,
+
+--     -- sorry,
+
+--     -- suffices : ∀ z ∈ (simulate cachingₛₒ (oa >>= ob) s).support,
+--     --   ⁅= fst z | simulate' cachingₛₒ (oa >>= ob) s⁆ ≤
+--     --     ⁅= fst z | simulate' cachingₛₒ (oa >>= ob) (f z)⁆,
+--     -- {
+
+--     -- }
+
+--     calc ⁅= (x, x) | simulate' cachingₛₒ (oa >>= ob) s >>= λ z,
+--         simulate' cachingₛₒ (oa >>= ob) s >>= λ z',
+--         return (z, z')⁆ =
+--       ⁅= (x, x) | (simulate cachingₛₒ oa s >>= λ x,
+--         simulate' cachingₛₒ (ob x.1) x.2) >>= λ z,
+--         (simulate cachingₛₒ oa s >>= λ x',
+--         simulate' cachingₛₒ (ob x'.1) x'.2) >>= λ z',
+--         return (z, z')⁆ : by pairwise_dist_equiv
+
+--       ... = ⁅= (x, x) | simulate cachingₛₒ oa s >>= λ x,
+--         simulate' cachingₛₒ (ob x.1) x.2 >>= λ z,
+--         (simulate cachingₛₒ oa s >>= λ x',
+--         simulate' cachingₛₒ (ob x'.1) x'.2) >>= λ z',
+--         return (z, z')⁆ : by pairwise_dist_equiv
+
+--       ... = ⁅= (x, x) | simulate cachingₛₒ oa s >>= λ x,
+--         simulate' cachingₛₒ (ob x.1) x.2 >>= λ z,
+--         simulate cachingₛₒ oa s >>= λ x',
+--         simulate' cachingₛₒ (ob x'.1) x'.2 >>= λ z',
+--         return (z, z')⁆ : by pairwise_dist_equiv
+
+--       ... = ⁅= (x, x) | simulate cachingₛₒ oa s >>= λ x,
+--         simulate cachingₛₒ (ob x.1) x.2 >>= λ z,
+--         simulate cachingₛₒ oa s >>= λ x',
+--         simulate' cachingₛₒ (ob x'.1) x'.2 >>= λ z',
+--         return (z.1, z')⁆ : by pairwise_dist_equiv
+
+--       ... ≤ ⁅= (x, x) | simulate cachingₛₒ oa s >>= λ x,
+--         simulate cachingₛₒ (ob x.1) x.2 >>= λ z,
+--         simulate cachingₛₒ oa (f z) >>= λ x',
+--         simulate' cachingₛₒ (ob x'.1) x'.2 >>= λ z',
+--         return (z.1, z')⁆ :
+--           begin
+
+--           end
+
+--       ... = ⁅= (x, x) | (simulate cachingₛₒ oa s >>= λ x,
+--         simulate cachingₛₒ (ob x.1) x.2) >>= λ z,
+--         simulate cachingₛₒ oa (f z) >>= λ x',
+--         simulate' cachingₛₒ (ob x'.1) x'.2 >>= λ z',
+--         return (z.1, z')⁆ : by pairwise_dist_equiv
+
+--       ... = ⁅= (x, x) | simulate cachingₛₒ (oa >>= ob) s >>= λ z,
+--         simulate' cachingₛₒ (oa >>= ob) (f z) >>= λ z',
+--         return (z.1, z')⁆ : begin
+--           pairwise_dist_equiv,
+--           refine trans (by pairwise_dist_equiv) (bind_dist_equiv_bind_of_dist_equiv_left _ _ _
+--             (simulate'_bind_dist_equiv _ _ _ _)).symm,
+--         end
+--   },
+--   {
+--     simp [simulate_query, simulate'_query],
+--     by_cases hs : s.is_fresh i t,
+--     {
+--       simp [hs],
+--       sorry,
+--     },
+--     {
+--       rw [not_is_fresh_iff_is_cached] at hs,
+--       have : f ((s.lookup i t).get_or_else default, s) = s := sorry,
+--       simp only [hs, this, get_or_else_of_is_cached],
+--       sorry,
+--     }
+--   }
+
+
+-- end
+
 end cachingₛₒ
 
-namespace sim_oracle
+-- namespace sim_oracle
 
-class is_resettable {S : Type} [has_bot S]
-  (so : sim_oracle spec spec' S) (so' : sim_oracle spec spec' S) :=
-(apply_bind_fst_map_apply_dist_equiv (i i' : spec.ι) (t : spec.domain i) (t' : spec.domain i')
-  (s : S) : do {x ← so i' (t', s), fst <$> so' i (t, x.2)} ≃ₚ fst <$> so' i (t, s) )
+-- class is_resettable {S : Type} [has_bot S]
+--   (so : sim_oracle spec spec' S) (so' : sim_oracle spec spec' S) :=
+-- (apply_bind_fst_map_apply_dist_equiv (i i' : spec.ι) (t : spec.domain i) (t' : spec.domain i')
+--   (s : S) : do {x ← so i' (t', s), fst <$> so' i (t, x.2)} ≃ₚ fst <$> so' i (t, s) )
 
-instance cachingₛₒ_is_resettable : is_resettable (@cachingₛₒ spec) cachingₛₒ :=
-{
-  apply_bind_fst_map_apply_dist_equiv := λ i i' t t' s,
-    cachingₛₒ.fst_map_apply_bind_apply_dist_equiv' _ _ _ _ _
-}
+-- instance cachingₛₒ_is_resettable : is_resettable (@cachingₛₒ spec) cachingₛₒ :=
+-- {
+--   apply_bind_fst_map_apply_dist_equiv := λ i i' t t' s,
+--     cachingₛₒ.fst_map_apply_bind_apply_dist_equiv' _ _ _ _ _
+-- }
 
-class is_rewinding {S : Type} [preorder S]
-  (so : sim_oracle spec spec' S) (so' : sim_oracle spec spec' S) :=
-(thing {α : Type} (oa : oracle_comp spec α) (i : spec.ι) (t : spec.domain i)
-  (s : S) (f : α × S → S) (hf : ∀ (x : α × S), s ≤ x.2 → s ≤ f x ∧ f x ≤ x.2) :
-  (simulate so oa s >>= λ x, so' i (t, f x)) ≃ₚ so' i (t, s))
+-- class is_rewinding {S : Type} [preorder S]
+--   (so : sim_oracle spec spec' S) (so' : sim_oracle spec spec' S) :=
+-- (thing {α : Type} (oa : oracle_comp spec α) (i : spec.ι) (t : spec.domain i)
+--   (s : S) (f : α × S → S) (hf : ∀ (x : α × S), s ≤ x.2 → s ≤ f x ∧ f x ≤ x.2) :
+--   (simulate so oa s >>= λ x, so' i (t, f x)) ≃ₚ so' i (t, s))
 
-instance cachingₛₒ_is_rewindable : is_rewinding (@cachingₛₒ spec) cachingₛₒ :=
-{
-  thing := begin
-    intros α oa i t s f hf,
-    induction oa using oracle_comp.induction_on with α a α β oa ob hoa hob i' t' generalizing s f hf,
-    {
-      simp [simulate_return],
-      refine trans (return_bind_dist_equiv _ _) _,
-      specialize hf (a, s) le_rfl,
-      have := le_antisymm hf.2 hf.1,
-      rw [this],
-    },
-    {
-      calc (simulate cachingₛₒ (oa >>= ob) s >>= λ y, cachingₛₒ i (t, f y)) ≃ₚ
-        (simulate cachingₛₒ oa s >>= λ x,
-          simulate cachingₛₒ (ob x.1) x.2) >>= λ y,
-          cachingₛₒ i (t, f y) : by pairwise_dist_equiv
-        ... ≃ₚ simulate cachingₛₒ oa s >>= λ x,
-          simulate cachingₛₒ (ob x.1) x.2 >>= λ y,
-          cachingₛₒ i (t, f y) : by pairwise_dist_equiv
-        ... ≃ₚ simulate cachingₛₒ oa s >>= λ x,
-          cachingₛₒ i (t, x.2) : begin
-            refine bind_dist_equiv_bind_of_dist_equiv_right _ _ _ (λ x hx, _),
-            refine hob x.1 x.2 f _,
-            sorry,
-          end
-        ... ≃ₚ cachingₛₒ i (t, s) : begin
-          refine hoa s prod.snd (λ x h, ⟨h, le_rfl⟩),
-        end
-    },
-    {
-      simp only [simulate_query, cachingₛₒ.apply_eq],
-      by_cases h : s.is_fresh i' t',
-      {
-        rw [get_or_else_of_is_fresh _ _ h],
-        refine trans (bind_map_dist_equiv _ _ _) _,
-        by_cases hi : i = i',
-        {
-          induction hi,
-          sorry,
-        },
-        {
-          refine trans (bind_dist_equiv_right _ _ default _) _,
-          sorry, sorry,
-        }
-      },
-      {
-        obtain ⟨u, hu⟩ := lookup_eq_some_of_is_cached _ (is_cached_of_not_is_fresh _ h),
-        rw [get_or_else_of_lookup_eq_some _ _ hu],
-        refine trans (return_bind_dist_equiv _ _) _,
-        specialize hf (u, s) le_rfl,
-        have := le_antisymm hf.2 hf.1,
-        rw [this],
-      }
-    }
-  end,
-}
+-- instance cachingₛₒ_is_rewindable : is_rewinding (@cachingₛₒ spec) cachingₛₒ :=
+-- {
+--   thing := begin
+--     intros α oa i t s f hf,
+--     induction oa using oracle_comp.induction_on with α a α β oa ob hoa hob i' t' generalizing s f hf,
+--     {
+--       simp [simulate_return],
+--       refine trans (return_bind_dist_equiv _ _) _,
+--       specialize hf (a, s) le_rfl,
+--       have := le_antisymm hf.2 hf.1,
+--       rw [this],
+--     },
+--     {
+--       calc (simulate cachingₛₒ (oa >>= ob) s >>= λ y, cachingₛₒ i (t, f y)) ≃ₚ
+--         (simulate cachingₛₒ oa s >>= λ x,
+--           simulate cachingₛₒ (ob x.1) x.2) >>= λ y,
+--           cachingₛₒ i (t, f y) : by pairwise_dist_equiv
+--         ... ≃ₚ simulate cachingₛₒ oa s >>= λ x,
+--           simulate cachingₛₒ (ob x.1) x.2 >>= λ y,
+--           cachingₛₒ i (t, f y) : by pairwise_dist_equiv
+--         ... ≃ₚ simulate cachingₛₒ oa s >>= λ x,
+--           cachingₛₒ i (t, x.2) : begin
+--             refine bind_dist_equiv_bind_of_dist_equiv_right _ _ _ (λ x hx, _),
+--             refine hob x.1 x.2 f _,
+--             sorry,
+--           end
+--         ... ≃ₚ cachingₛₒ i (t, s) : begin
+--           refine hoa s prod.snd (λ x h, ⟨h, le_rfl⟩),
+--         end
+--     },
+--     {
+--       simp only [simulate_query, cachingₛₒ.apply_eq],
+--       by_cases h : s.is_fresh i' t',
+--       {
+--         rw [get_or_else_of_is_fresh _ _ h],
+--         refine trans (bind_map_dist_equiv _ _ _) _,
+--         by_cases hi : i = i',
+--         {
+--           induction hi,
+--           sorry,
+--         },
+--         {
+--           refine trans (bind_dist_equiv_right _ _ default _) _,
+--           sorry, sorry,
+--         }
+--       },
+--       {
+--         obtain ⟨u, hu⟩ := lookup_eq_some_of_is_cached _ (is_cached_of_not_is_fresh _ h),
+--         rw [get_or_else_of_lookup_eq_some _ _ hu],
+--         refine trans (return_bind_dist_equiv _ _) _,
+--         specialize hf (u, s) le_rfl,
+--         have := le_antisymm hf.2 hf.1,
+--         rw [this],
+--       }
+--     }
+--   end,
+-- }
 
-end sim_oracle
+-- end sim_oracle
