src/computational_monads/simulation_semantics/simulate/product.lean
@@ -1,0 +1,25 @@
+/-
+Copyright (c) 2023 Devon Tuma. All rights reserved.
+Released under Apache 2.0 license as described in the file LICENSE.
+Authors: Devon Tuma
+-/
+import computational_monads.simulation_semantics.simulate.monad
+
+/-!
+# Distributional Semantics of Simulation of a Pair of Computations
+
+This file contains lemmas about simulation semantics interactions with `simulate`
+-/
+
+variables {α β γ : Type} {spec spec' : oracle_spec} {S : Type}
+
+namespace oracle_comp
+
+open oracle_spec
+open_locale big_operators ennreal
+
+variables (so : sim_oracle spec spec' S) (a : α) (s : S)
+
+-- lemma simulate'_product_dist_equiv
+
+end oracle_comp
